Source/DafnyStandardLibraries/src/Std/Actions/BulkActions.dfy
@@ -6,13 +6,23 @@ module Std.BulkActions {
   import opened Wrappers
   import opened BoundedInts
 
+  datatype OptionResult<T, E> = Good(value: T) | Bad(error: E) | Done
+
   @AssumeCrossModuleTermination
   trait BulkAction<I, O> extends Action<I, O> {
 
-    method BulkInvoke(input: Producer<I>, output: IConsumer<O>)
+    method BulkInvoke(input: Producer<I>, output: IConsumer<O>, outputTotalProof: TotalActionProof<O, ()>)
+      requires Valid()
       requires input.Valid()
       requires output.Valid()
-    
+      requires outputTotalProof.Valid()
+      requires outputTotalProof.Action() == output
+      requires Repr !! input.Repr !! output.Repr !! outputTotalProof.Repr
+      reads this, Repr, input, input.Repr, output, output.Repr, outputTotalProof, outputTotalProof.Repr
+      modifies Repr, input.Repr, output.Repr, outputTotalProof.Repr
+      ensures Valid()
+      ensures input.Valid()
+      ensures output.Valid()
   }
 
   // @AssumeCrossModuleTermination
@@ -24,12 +34,13 @@ module Std.BulkActions {
 
   // }
 
-  class Chunker<E> extends BulkAction<Option<Result<uint8, E>>, Option<Producer<Result<uint8, E>>>> {
+  class Chunker<E> extends BulkAction<Option<Result<uint8, E>>, Producer<Option<Result<uint8, E>>>> {
 
     const chunkSize: uint64
     var chunkBuffer: BoundedInts.bytes
 
     constructor(chunkSize: uint64)
+      requires 0 < chunkSize
       ensures Valid()
       ensures fresh(Repr)
       ensures history == []
@@ -46,16 +57,17 @@ module Std.BulkActions {
       ensures Valid() ==> ValidHistory(history)
       decreases Repr, 0
     {
-      this in Repr
+      && this in Repr
+      && 0 < chunkSize
     }
 
-    ghost predicate ValidHistory(history: seq<(Option<Result<uint8, E>>, Option<Producer<Result<uint8, E>>>)>)
+    ghost predicate ValidHistory(history: seq<(Option<Result<uint8, E>>, Producer<Option<Result<uint8, E>>>)>)
       decreases Repr
     {
       true
     }
 
-    ghost predicate ValidInput(history: seq<(Option<Result<uint8, E>>, Option<Producer<Result<uint8, E>>>)>, next: Option<Result<uint8, E>>)
+    ghost predicate ValidInput(history: seq<(Option<Result<uint8, E>>, Producer<Option<Result<uint8, E>>>)>, next: Option<Result<uint8, E>>)
       requires ValidHistory(history)
       decreases Repr
     {
@@ -66,7 +78,15 @@ module Std.BulkActions {
       // MappedProducer could actually wrap an IProducer instead
       // and just prove that it eventually produces None?
       // Probably IMappedProducer or something instead)
-      true
+      //
+      // Tricky part of BulkInvoke is it's meant to be delivering a batch of values,
+      // and None means end of batch, not end of all input.
+      // Something like a Chunker needs an EOI to flush buffered values
+      // (or produce an error!)
+      // Options:
+      //  * Mapped(input, action) + Something(action)
+      //  * Mapped(LiftAndAddEOI(input), action) - Three-state data/error/done datatype?
+      Seq.Partitioned(InputsOf(history) + [next], IsSome)
     }
 
     ghost function Decreases(i: Option<Result<uint8, E>>): ORDINAL
@@ -76,7 +96,7 @@ module Std.BulkActions {
       0
     }
 
-    method Invoke(i: Option<Result<uint8, E>>) returns (o: Option<Producer<Result<uint8, E>>>)
+    method Invoke(i: Option<Result<uint8, E>>) returns (o: Producer<Option<Result<uint8, E>>>)
       requires Requires(i)
       reads Reads(i)
       modifies Modifies(i)
@@ -85,68 +105,129 @@ module Std.BulkActions {
     {
       var input := new SeqReader([i]);
       var output := new SeqWriter();
-      BulkInvoke(input, output);
+      var outputTotalProof := new SeqWriterTotalActionProof(output);
+      BulkInvoke(input, output, outputTotalProof);
       o := output.values[0];
     }
 
     
+    function ToOptionResult<T, E>(t: T): Option<Result<T, E>> {
+      Some(Success(t))
+    }
 
-    method CollectToSeqResult<T, E>(p: Producer<Result<T, E>>) returns (r: Result<seq<T>, E>)
+    method ToOptionResultProducer<T, E>(values: seq<T>) returns (result: Producer<Option<Result<T, E>>>)
+      reads {}
+      ensures result.Valid()
+      ensures fresh(result.Repr)
+      ensures result.history == []
+    {
+      var chunkProducer := new SeqReader(values);
+      var mapping := new FunctionAction(ToOptionResult);
+      var mappingTotalProof := new TotalFunctionActionProof(mapping);
+      result := new MappedProducer(chunkProducer, mapping, mappingTotalProof);
+    }
+
+    // TODO: Consider dedicated three-state datatype instead of Option<Result<...>>
+    // Result is all values produced, plus the terminal state: 
+    // normal (Success(true)), EOI (Success(false)) or error (Failure(error))
+    method CollectToSeqResult<T, E>(p: Producer<Option<Result<T, E>>>) returns (values: seq<T>, state: Result<bool, E>)
       requires p.Valid()
-      ensures p.Valid()
+      reads p, p.Repr
+      modifies p.Repr
+      ensures p.ValidAndDisjoint()
       ensures p.Done()
 
     {
-      if p is MappedProducer {
-        // TODO: optimization
-      }
+      // TODO: optimization - needs duplicate class to get around lack of compiled is
+      // if p is MappedProducer<T, Option<Result<T, E>>> {
+      //   var mp := p as MappedProducer;
+      //   if mp.mapping is FunctionAction<T, Option<Result<T, E>>> {
+      //     values := CollectToSeq(mp.original);
+      //     state := Success(true);
+      //     return;
+      //   }
+      // }
 
-      var s := CollectToSeq(p);
-      var optIndex := Seq.IndexByOption(s, (x: Result<T, E>) => x.Failure?);
-      match optIndex {
-        case Some(index) =>
-          r := Failure(s[index].error);
-        case None =>
-          r := Success(Seq.Map((x: Result<T, E>) => x.value, s));
+      values := [];
+      state := Success(true);
+      while true 
+        invariant fresh(p.Repr - old(p.Repr))
+        invariant p.Valid()
+        decreases p.Remaining()
+      {
+        var next := p.Next();
+        if next.None? {
+          assert Seq.Last(p.Outputs()) == None;
+          assert p.Done();
+          break;
+        }
+
+        match next.value {
+          case Some(Success(t)) => values := values + [t];
+          case Some(Failure(e)) => state := Failure(e);
+          case None => state := Success(false);
+        }
       }
+      assert p.Done();
     }
 
-    method BulkInvoke(input: Producer<Option<Result<uint8, E>>>, output: IConsumer<Option<Producer<Result<uint8, E>>>>)
+    @ResourceLimit("0")
+    method BulkInvoke(input: Producer<Option<Result<uint8, E>>>, 
+                      output: IConsumer<Producer<Option<Result<uint8, E>>>>,
+                      outputTotalProof: TotalActionProof<Producer<Option<Result<uint8, E>>>, ()>)
+      requires Valid()
       requires input.Valid()
       requires output.Valid()
+      requires outputTotalProof.Valid()
+      requires outputTotalProof.Action() == output
+      requires Repr !! input.Repr !! output.Repr !! outputTotalProof.Repr
+      reads this, Repr, input, input.Repr, output, output.Repr, outputTotalProof, outputTotalProof.Repr
+      modifies Repr, input.Repr, output.Repr, outputTotalProof.Repr
+      ensures Valid()
+      ensures input.Valid()
+      ensures output.Valid()
     {
       assert Valid();
-      var outputChunks := [];
 
-      var inputSeq := CollectToSeqResult(input);
+      var inputSeq, state := CollectToSeqResult(input);
+      chunkBuffer := chunkBuffer + inputSeq;
+        
+      while chunkSize as int <= |chunkBuffer|
+        invariant fresh(Repr - old(Repr))
+        invariant Valid()
+        invariant fresh(input.Repr - old(input.Repr))
+        invariant input.Valid()
+        invariant fresh(output.Repr - old(output.Repr))
+        invariant output.Valid()
+        invariant fresh(outputTotalProof.Repr - old(outputTotalProof.Repr))
+        invariant outputTotalProof.Valid()
+        invariant Repr !! input.Repr !! output.Repr !! outputTotalProof.Repr
+        invariant history == old(history)
+        decreases |chunkBuffer|
+      {
+        var nextChunk := chunkBuffer[..chunkSize];
+        chunkBuffer := chunkBuffer[chunkSize..];
 
-      if input.Some? {
-        if input.value.Failure? {
-          outputChunks := outputChunks + [input.value];
-        } else {
-
-          chunkBuffer := chunkBuffer + input.value.value;
-          
-          while chunkSize as int <= |chunkBuffer|
-            invariant ValidAndDisjoint()
-            invariant history == old(history)
-          {
-            outputChunks := outputChunks + [Success(chunkBuffer[..chunkSize])];
-            chunkBuffer := chunkBuffer[chunkSize..];
-          }
-        }
-      } else {
-        if 0 < |chunkBuffer| {
-          outputChunks := outputChunks + [Success(chunkBuffer)];
-        } else {
-          r := None;
-          UpdateHistory(input, r);
-          return;
-        }
+        var chunkProducer := ToOptionResultProducer(nextChunk);
+        outputTotalProof.AnyInputIsValid(output.history, chunkProducer);
+        output.Accept(chunkProducer);
       }
-      var output := new SeqReader(outputChunks);
-      r := Some(output);
-      UpdateHistory(input, r);
+
+      match state {
+      case Failure(error) =>
+        var errorProducer := new SeqReader([Some(Failure(error))]);
+        outputTotalProof.AnyInputIsValid(output.history, errorProducer);
+        output.Accept(errorProducer);
+      case Success(false) =>
+        if 0 < |chunkBuffer| {
+          // To make it more interesting, produce an error if outputChunks is non empty?
+          var nextChunk := chunkBuffer;
+          var chunkProducer := ToOptionResultProducer(nextChunk);
+          outputTotalProof.AnyInputIsValid(output.history, chunkProducer);
+          output.Accept(chunkProducer);
+        }
+      case Success(true) => {}
+      }
     }
   }
 
